Add and use a new wfe judgment in the Coq model.

src/coq/Dot_Rules.v
@@ -80,11 +80,11 @@ Inductive typing : env -> tm -> tp -> Prop :=
       E |= T' ~<: S ->
       E |= (app t t') ~: T
   | typing_abs : forall L E S t T,
-      wf_tp E S ->
+      wfe_tp E S ->
       (forall x, x \notin L -> (ctx_bind E x S) |= (t ^ x) ~: T) ->
       E |= (lam S t) ~: (tp_fun S T)
   | typing_new : forall L E Tc args t T' ds,
-      wf_tp E Tc ->
+      wfe_tp E Tc ->
       concrete Tc ->
       E |= Tc ~< ds ->
       lbl.uniq args ->
@@ -214,20 +214,20 @@ with sub_decl : env -> decl -> decl -> Prop :=
 with wf_tp : env -> tp -> Prop :=
   | wf_rfn : forall L E T DS,
       decls_ok (decls_fin DS) ->
-      wf_tp E T ->
+      wfe_tp E T ->
       (forall z, z \notin L ->
         forall l d, decls_binds l d (decls_fin DS) -> (wf_decl (ctx_bind E z (tp_rfn T DS)) (d ^d^ z))) ->
       wf_tp E (tp_rfn T DS)
   | wf_fun : forall E T1 T2,
-      wf_tp E T1 ->
-      wf_tp E T2 ->
+      wfe_tp E T1 ->
+      wfe_tp E T2 ->
       wf_tp E (tp_fun T1 T2)
   | wf_tsel_1 : forall E p L S U,
       path p ->
       type_label L ->
       E |= p ~mem~ L ~: (decl_tp S U) ->
-      wf_tp E S ->
-      wf_tp E U ->
+      wfe_tp E S ->
+      wfe_tp E U ->
       wf_tp E (tp_sel p L)
   | wf_tsel_2 : forall E p L U,
       path p ->
@@ -235,12 +235,12 @@ with wf_tp : env -> tp -> Prop :=
       E |= p ~mem~ L ~: (decl_tp tp_bot U) ->
       wf_tp E (tp_sel p L)
   | wf_and : forall E T1 T2,
-      wf_tp E T1 ->
-      wf_tp E T2 ->
+      wfe_tp E T1 ->
+      wfe_tp E T2 ->
       wf_tp E (tp_and T1 T2)
   | wf_or : forall E T1 T2,
-      wf_tp E T1 ->
-      wf_tp E T2 ->
+      wfe_tp E T1 ->
+      wfe_tp E T2 ->
       wf_tp E (tp_or T1 T2)
   | wf_bot : forall E,
       wf_tp E tp_bot
@@ -249,12 +249,18 @@ with wf_tp : env -> tp -> Prop :=
 
 with wf_decl : env -> decl -> Prop :=
   | wf_decl_tp : forall E S U,
-      wf_tp E S ->
-      wf_tp E U ->
+      wfe_tp E S ->
+      wfe_tp E U ->
       wf_decl E (decl_tp S U)
   | wf_decl_tm : forall E T,
-      wf_tp E T ->
+      wfe_tp E T ->
       wf_decl E (decl_tm T)
+
+with wfe_tp : env -> tp -> Prop :=
+  | wfe_any : forall E T DT,
+      wf_tp E T ->
+      E |= T ~< DT ->
+      wfe_tp E T
 .
 
 (* ********************************************************************** *)
@@ -266,21 +272,24 @@ Scheme typing_indm         := Induction for typing Sort Prop
   with sub_tp_indm         := Induction for sub_tp Sort Prop
   with sub_decl_indm       := Induction for sub_decl Sort Prop
   with wf_tp_indm          := Induction for wf_tp Sort Prop
-  with wf_decl_indm        := Induction for wf_decl Sort Prop.
+  with wf_decl_indm        := Induction for wf_decl Sort Prop
+  with wfe_tp_indm         := Induction for wfe_tp Sort Prop
+.
 
-Combined Scheme typing_mutind from typing_indm, mem_indm, expands_indm, sub_tp_indm, sub_decl_indm, wf_tp_indm, wf_decl_indm.
+Combined Scheme typing_mutind from typing_indm, mem_indm, expands_indm, sub_tp_indm, sub_decl_indm, wf_tp_indm, wf_decl_indm, wfe_tp_indm.
 
 Require Import LibTactics_sf.
-Ltac mutind_typing P0_ P1_ P2_ P3_ P4_ P5_ P6_ :=
+Ltac mutind_typing P0_ P1_ P2_ P3_ P4_ P5_ P6_ P7_ :=
   cut ((forall E t T (H: E |= t ~: T), (P0_ E t T H)) /\ 
   (forall E t l d (H: E |= t ~mem~ l ~: d), (P1_ E t l d H)) /\
   (forall E T DS (H: E |= T ~< DS), (P2_ E T DS H)) /\ 
   (forall E T T' (H: E |= T ~<: T'), (P3_  E T T' H))  /\ 
   (forall (e : env) (d d' : decl) (H : sub_decl e d d'), (P4_ e d d' H)) /\  
   (forall (e : env) (t : tp) (H : wf_tp e t), (P5_ e t H)) /\  
-  (forall (e : env) (d : decl) (H : wf_decl e d), (P6_ e d H))); [tauto | 
-    apply (typing_mutind P0_ P1_ P2_ P3_ P4_ P5_ P6_); try unfold P0_, P1_, P2_, P3_, P4_, P5_, P6_ in *; try clear P0_ P1_ P2_ P3_ P4_ P5_ P6_; [  (* only try unfolding and clearing in case the PN_ aren't just identifiers *)
-      Case "typing_var" | Case "typing_ref" | Case "typing_sel" | Case "typing_app" | Case "typing_abs" | Case "typing_new" | Case "mem_path" | Case "mem_term" | Case "expands_rfn" | Case "expands_tsel" | Case "expands_and" | Case "expands_or" | Case "expands_top" | Case "expands_fun" | Case "expands_bot" | Case "sub_tp_refl" | Case "sub_tp_fun" | Case "sub_tp_rfn_r" | Case "sub_tp_rfn_l" | Case "sub_tp_tsel_r" | Case "sub_tp_tsel_l" | Case "sub_tp_and_r" | Case "sub_tp_and_l1" | Case "sub_tp_and_l2" | Case "sub_tp_or_r1" | Case "sub_tp_or_r2" | Case "sub_tp_or_l" | Case "sub_tp_top" | Case "sub_tp_bot" | Case "sub_decl_tp" | Case "sub_decl_tm" | Case "wf_rfn" | Case "wf_fun" | Case "wf_tsel_1" | Case "wf_tsel_2" | Case "wf_and" | Case "wf_or" | Case "wf_bot" | Case "wf_top" | Case "wf_decl_tp" | Case "wf_decl_tm" ]; 
+  (forall (e : env) (d : decl) (H : wf_decl e d), (P6_ e d H)) /\
+  (forall (e : env) (t : tp) (H : wfe_tp e t), (P7_ e t H))); [tauto | 
+    apply (typing_mutind P0_ P1_ P2_ P3_ P4_ P5_ P6_); try unfold P0_, P1_, P2_, P3_, P4_, P5_, P6_, P7_ in *; try clear P0_ P1_ P2_ P3_ P4_ P5_ P6_; [  (* only try unfolding and clearing in case the PN_ aren't just identifiers *)
+      Case "typing_var" | Case "typing_ref" | Case "typing_sel" | Case "typing_app" | Case "typing_abs" | Case "typing_new" | Case "mem_path" | Case "mem_term" | Case "expands_rfn" | Case "expands_tsel" | Case "expands_and" | Case "expands_or" | Case "expands_top" | Case "expands_fun" | Case "expands_bot" | Case "sub_tp_refl" | Case "sub_tp_fun" | Case "sub_tp_rfn_r" | Case "sub_tp_rfn_l" | Case "sub_tp_tsel_r" | Case "sub_tp_tsel_l" | Case "sub_tp_and_r" | Case "sub_tp_and_l1" | Case "sub_tp_and_l2" | Case "sub_tp_or_r1" | Case "sub_tp_or_r2" | Case "sub_tp_or_l" | Case "sub_tp_top" | Case "sub_tp_bot" | Case "sub_decl_tp" | Case "sub_decl_tm" | Case "wf_rfn" | Case "wf_fun" | Case "wf_tsel_1" | Case "wf_tsel_2" | Case "wf_and" | Case "wf_or" | Case "wf_bot" | Case "wf_top" | Case "wf_decl_tp" | Case "wf_decl_tm" | Case "wfe_any" ]; 
       introv; eauto ].
 
 
@@ -293,6 +302,7 @@ Section TestMutInd.
   Let Psbd (E: env) (d d': decl) (H: sub_decl E d d') := True.
   Let Pwft (E: env) (t: tp) (H: wf_tp E t) := True.
   Let Pwfd (E: env) (d: decl) (H: wf_decl E d) := True.
+  Let Pwfe (E: env) (t: tp) (H: wfe_tp E t) := True.
 Lemma EnsureMutindTypingTacticIsUpToDate : True. 
-Proof. mutind_typing Ptyp Pmem Pexp Psub Psbd Pwft Pwfd; intros; auto. Qed.
+Proof. mutind_typing Ptyp Pmem Pexp Psub Psbd Pwft Pwfd Pwfe; intros; auto. Qed.
 End TestMutInd.
